Prove everything

ExamplePrograms.thy
@@ -92,7 +92,7 @@ definition mult_body_pre :: "precondition" where
   \<and> 0 \<le>s i
   \<and> i <s b
   \<and> b \<le>s 2 ^ 31 - 1
-  \<and> i <s 2 ^ 31 - 1
+  \<and> i \<le>s 2 ^ 31 - 1
   )"
 
 (*
@@ -148,7 +148,7 @@ definition mult_end_pre :: "precondition" where
   \<and> sint a * sint b \<le> 2 ^ 31 - 1
   \<and> 0 <s b
   \<and> 0 \<le>s i
-  \<and> i <s 2 ^ 31 - 1
+  \<and> i \<le>s 2 ^ 31 - 1
   \<and> i = b
   )"
 
@@ -223,8 +223,133 @@ method unfold_wp_steps_until =
   (unfold_wp_step | unfold_endgoal)?
 
 
-lemma i_no_overflow_impl_positive: "0 \<le>s i \<Longrightarrow> (i::word32) <s 2^31 - 1 \<Longrightarrow> 0 \<le>s (i+1)"
-  sorry
+
+lemma lt_imp_le: "(i::word32) <s 2 ^ 31 - 1 \<Longrightarrow> i \<le>s 2 ^ 31 - 2"
+  by (simp add: word_sle_eq word_sless_alt)
+lemma le_imp_lt: "i \<le>s 2 ^ 31 - 2 \<Longrightarrow> (i::word32) <s 2 ^ 31 - 1"
+  by (simp add: word_sle_eq word_sless_alt)
+
+lemma lt_inc_nlt_imp_eq[simp]: "(i::word32) <s (b::word32) \<Longrightarrow> \<not> i+1 <s b \<Longrightarrow> i+1 = b"
+  apply (simp add: word_sle_eq word_sless_alt)
+  by (smt (verit, ccfv_threshold) diff_add_cancel signed_arith_ineq_checks_to_eq_word32(1,2) signed_minus_1
+      signed_take_bit_int_eq_self signed_take_bit_int_greater_eq_minus_exp sint_word_ariths(1,8) word_sint.Rep_eqD)
+
+lemma i_no_overflow_impl_positive[simp]: "0 \<le>s i \<Longrightarrow> (i::word32) <s 2^31 - 1 \<Longrightarrow> 0 \<le>s (i+1)"
+  by (smt (verit, del_insts) add_diff_eq diff_add_cancel diff_numeral_special(10) of_int_eq_id signed_minus_1
+      signed_take_bit_int_eq_self signed_take_bit_int_eq_self_iff signed_take_bit_int_greater_eq_minus_exp sint_word_ariths(1,2,8)
+      word_sle_eq word_sless_alt)
+
+lemma i_bounds_no_overflow_neg[simp]: "- (2 ^ 31) \<le> sint (a::word32) * sint (b::word32) \<Longrightarrow>
+    sint a * sint b \<le> 2 ^ 31 - 1 \<Longrightarrow>
+    0 \<le>s (i::word32) \<Longrightarrow>
+    i <s b \<Longrightarrow>
+    b \<le>s 2 ^ 31 - 1 \<Longrightarrow>
+    i <s 2 ^ 31 - 1 \<Longrightarrow>
+    a <s 0 \<Longrightarrow> a * i <s 0 \<Longrightarrow> \<not> 0 \<le>s a * i + a"
+proof -
+  assume bounds: "- (2^31) \<le> sint a * sint b" "sint a * sint b \<le> 2^31 - 1"
+  assume hi: "0 \<le>s i" "i <s b" "b \<le>s 2^31 - 1" "i <s 2^31 - 1"
+  assume neg: "a <s 0" "a * i <s 0"
+  have sa: "sint a < 0"
+    using neg(1) 
+    by (simp add: word_sless_alt)
+  have si: "0 \<le> sint i"
+    using hi(1)
+    by (simp add: word_sless_alt word_sle_eq)
+  have si_lt: "sint i < 2^31 - 1"
+    using hi(4) by (simp add: word_sless_alt word_sle_eq)
+  have sb_lt: "sint b \<le> 2^31 - 1"
+    using hi(3) by (simp add: word_sless_alt word_sle_eq)
+  have sai_neg: "sint (a * i) < 0"
+    using neg(2) by (simp add: word_sless_alt word_sle_eq)
+  have no_ovf_ai: "sint (a * i) = sint a * sint i"
+    using sai_neg sa si 
+    apply(auto intro: signed_arith_sint simp: sint_word_ariths word_sless_alt word_sle_eq)
+    by (smt (verit, del_insts) bounds(1) hi(2) mult_eq_0_iff mult_less_cancel_left_disj signed_take_bit_int_eq_self
+        word_sless_alt)
+  have no_ovf_sum: "sint (a * i + a) = sint (a * i) + sint a"
+    proof -
+      have lo: "-(2^31) \<le> sint (a * i) + sint a"
+      proof -
+        have si_lt_b: "sint i < sint b"
+          using hi(2) by (simp add: word_sless_alt)
+        have sb_bounds: "-(2^31) \<le> sint b"
+          using si si_lt_b by auto
+        have key: "sint a * sint b \<le> sint a * (sint i + 1)"
+          using sa si_lt_b
+          by (simp add: mult_le_cancel_left_neg)
+        show ?thesis
+          using no_ovf_ai key bounds(1) right_diff_distrib' mult_cancel_left2
+          by (smt (verit) )
+      qed
+      have hi': "sint (a * i) + sint a \<le> 2^31 - 1"
+        using sai_neg sa
+        by simp
+      then show ?thesis
+        using lo hi' no_ovf_ai
+        by (simp add: sint_word_ariths signed_take_bit_int_eq_self)
+    qed
+  show "\<not> 0 \<le>s a * i + a"
+    unfolding word_sle_def
+    using no_ovf_sum sai_neg sa
+    by (smt (verit) neg(1) word_sle_def word_sle_eq word_sless_alt)
+qed
+
+lemma i_bounds_no_overflow_pos[simp]: "- (2 ^ 31) \<le> sint (a::word32) * sint (b::word32) \<Longrightarrow>
+    sint a * sint b \<le> 2 ^ 31 - 1 \<Longrightarrow>
+    0 <s b \<Longrightarrow>
+    0 \<le>s (i::word32) \<Longrightarrow>
+    i <s b \<Longrightarrow>
+    b \<le>s 2 ^ 31 - 1 \<Longrightarrow>
+    i <s 2 ^ 31 - 1 \<Longrightarrow>
+    0 \<le>s a \<Longrightarrow> 0 \<le>s a * i \<Longrightarrow> \<not>  a * i + a <s 0"
+proof -
+  assume bounds: "- (2^31) \<le> sint a * sint b" "sint a * sint b \<le> 2^31 - 1"
+  assume hi: "0 \<le>s i" "i <s b" "b \<le>s 2^31 - 1" "i <s 2^31 - 1"
+  assume pos: "0 \<le>s a" "0 \<le>s a * i"
+  have sa: "sint a \<ge> 0"
+    using pos(1)
+    by (simp add: word_sle_eq)
+  have si: "0 \<le> sint i"
+    using hi(1)
+    by (simp add: word_sless_alt word_sle_eq)
+  have si_lt: "sint i < 2^31 - 1"
+    using hi(4) by (simp add: word_sless_alt word_sle_eq)
+  have sb_lt: "sint b \<le> 2^31 - 1"
+    using hi(3) by (simp add: word_sless_alt word_sle_eq)
+  have sai_neg: "sint (a * i) \<ge> 0"
+    using pos(2) by (simp add: word_sless_alt word_sle_eq)
+  have no_ovf_ai: "sint (a * i) = sint a * sint i"
+    using sai_neg sa si 
+    apply(auto intro: signed_arith_sint simp: sint_word_ariths word_sless_alt word_sle_eq)
+    by (smt (verit, best) bounds(2) hi(2) mult_less_cancel_left_disj signed_take_bit_int_eq_self word_sless_alt
+        zero_le_mult_iff)
+  have no_ovf_sum: "sint (a * i + a) = sint (a * i) + sint a"
+    proof -
+      have lo: "-(2^31) \<le> sint (a * i) + sint a"
+        using sa sai_neg by force
+      have hi': "sint (a * i) + sint a \<le> 2^31 - 1"
+      proof -
+        have si_lt_b: "sint i < sint b"
+          using hi(2) by (simp add: word_sless_alt)
+        have sb_bounds: "-(2^31) \<le> sint b"
+          using si si_lt_b by auto
+        have key: "sint a * sint b \<ge> sint a * (sint i + 1)"
+          using sa si_lt_b
+          by (smt (verit, best) mult_less_cancel_left_disj)
+        show ?thesis
+          using no_ovf_ai key bounds(2) right_diff_distrib' mult_cancel_left2
+          by (smt (verit, best))
+      qed
+      then show ?thesis
+        using lo hi' no_ovf_ai
+        by (simp add: sint_word_ariths signed_take_bit_int_eq_self)
+    qed
+  show ?thesis
+    unfolding word_sle_def
+    using no_ovf_sum sai_neg sa 
+    by (smt (verit) pos(1) word_sle_def word_sle_eq word_sless_alt)
+qed
 
 
 lemma
@@ -246,21 +371,20 @@ lemma
     apply (unfold_wp_steps_until)
     apply (unfold mult_body_pre_def)
     apply (unfold_shorthands)
-    apply (intro conjI exI) apply auto by (auto split: if_splits)
+    apply (intro exI) apply (rule conjI) apply simp apply (rule conjI, simp) apply (rule conjI)
+    apply (intro exI) apply (rule conjI) apply simp by auto
 
   subgoal for s (* body \<rightarrow> inc \<rightarrow> cond \<rightarrow> body or end *)
     apply (unfold_wp_annotated_step)
-    apply (block_vcg_dbg defs: mult_body_def mult_body_pre_def)
-    subgoal sorry
-    subgoal sorry
-    apply (block_vcg)
+    apply (block_vcg defs: mult_body_def mult_body_pre_def)
     apply (unfold_wp_steps_until)
     apply (block_vcg_dbg defs: mult_inc_def)
-    subgoal sorry
+    subgoal using i_no_overflow_impl_positive word_sle_eq word_sless_alt
+      by (smt (verit, best))
     apply block_vcg
     apply (unfold_wp_steps_until)
     apply (block_vcg defs: mult_cond_def)
-    subgoal
+    subgoal (* cond \<rightarrow> body *)
       apply (rule wp_steps_until_intro)
       defer
       unfolding has_annotation_def apply simp
@@ -269,17 +393,18 @@ lemma
       apply (rule exI) apply (intro conjI) apply simp
       apply (rule exI) apply (intro conjI) apply simp apply simp apply simp
       apply (rule exI) apply (rule conjI, simp)+
-      apply (metis distrib_left mult.right_neutral) apply (rule conjI, simp)+ using i_no_overflow_impl_positive by auto
-    subgoal for a b i aa ab ac ad ae af ag ah ai aj ak al am an 
+      apply (metis distrib_left mult.right_neutral) apply (rule conjI, simp)+ by simp
+    subgoal (* cond \<longrightarrow> end *)
       apply (rule wp_steps_until_intro)
       defer
       unfolding has_annotation_def apply simp
       unfolding annotation_holds_def
       apply (simp (no_asm)) unfolding mult_end_pre_def apply unfold_shorthands
       apply (rule exI | rule conjI, simp)+
-       apply (metis distrib_left mult.right_neutral) apply (rule conjI, simp)+
-      subgoal sorry
-      subgoal sorry
+      subgoal using lt_inc_nlt_imp_eq distrib_left mult_numeral_1_right numeral_One
+        by (metis (no_types, lifting) )
+      subgoal using lt_inc_nlt_imp_eq
+        by force
       done
     done
 
